SEARsettings.sml
@@ -2258,6 +2258,8 @@ e0
 
 
 
+
+
 val o_Eval' = o_Eval |> strip_all_and_imp |> gen_all
                      |> disch_all |> gen_all
                      |>store_as "o_Eval'"
@@ -3236,3 +3238,21 @@ val it =
     ["(z -> psv  2)", "(y -> psv  0)", "(a -> psv  1)"], [], 3):
    string list * string list * string list * string list * int
 *)
+
+val Fst_ex = prove_store("Fst_ex",
+e0
+(rpt strip_tac >> qexists_tac ‘Eval(p1(A,B),x)’ >> rw[])
+(form_goal
+ “!A B x:mem(A * B).?fstx. Eval(p1(A,B),x) = fstx”));
+
+ 
+val Snd_ex = prove_store("Snd_ex",
+e0
+(rpt strip_tac >> qexists_tac ‘Eval(p2(A,B),x)’ >> rw[])
+(form_goal
+ “!A B x:mem(A * B).?sndx. Eval(p2(A,B),x) = sndx”));
+
+val Fst_def = Fst_ex |> spec_all |> ex2fsym0 "Fst" ["x"]
+val Snd_def = Snd_ex |> spec_all |> ex2fsym0 "Snd" ["x"]
+
+val Pair_def' = Pair_def |> rewr_rule[Fst_def,Snd_def]
